src/CFG/Collecting/CFG_Collect_IP.thy
@@ -1,0 +1,176 @@
+theory CFG_Collect_IP
+  imports CFG_Edges_Collect IMP2_Proc_to_CFG
+begin
+
+(*
+  Interprocedural collecting semantics (M1 slice 2).
+
+  Extends cfg_collect with combine triples from combines g:
+    (call, proc_exit, return) contributes
+      { combine_states s t | s in C call, t in C proc_exit }
+    at the return program point.
+
+  When combines g = {}, agrees with cfg_collect.
+  Operational adequacy (pruns_to => cfg_collect_ip) is the next proof target.
+*)
+
+definition collect_combine_pp :: "cfg \<Rightarrow> cenv \<Rightarrow> pp \<Rightarrow> store set" where
+  "collect_combine_pp g rho v =
+     \<Union>{ {combine_states s t | s t. s \<in> rho c \<and> t \<in> rho ex}
+           | c ex ret. (c, ex, ret) \<in> combines g \<and> ret = v }"
+
+definition cfg_collect_ip_F :: "cfg \<Rightarrow> store set \<Rightarrow> cenv \<Rightarrow> cenv" where
+  "cfg_collect_ip_F g S rho v =
+     (if v = cfg_entry g then S else {})
+     \<union> collect_pp g rho v
+     \<union> collect_combine_pp g rho v"
+
+definition cfg_collect_ip :: "cfg \<Rightarrow> store set \<Rightarrow> cenv" where
+  "cfg_collect_ip g S = lfp (cfg_collect_ip_F g S)"
+
+(* -- Monotonicity ------------------------------------------------ *)
+
+lemma combine_states_image_mono:
+  assumes "S \<subseteq> S'" and "T \<subseteq> T'"
+  shows "{combine_states s t | s t. s \<in> S \<and> t \<in> T}
+         \<subseteq> {combine_states s t | s t. s \<in> S' \<and> t \<in> T'}"
+  using assms by blast
+
+lemma collect_combine_pp_mono:
+  "mono (\<lambda>rho. collect_combine_pp g rho v)"
+proof
+  fix rho1 rho2 :: cenv
+  assume le: "rho1 \<le> rho2"
+  have sub: "\<And>u. rho1 u \<subseteq> rho2 u"
+    using le unfolding le_fun_def by auto
+  show "collect_combine_pp g rho1 v \<subseteq> collect_combine_pp g rho2 v"
+  proof
+    fix x
+    assume xin: "x \<in> collect_combine_pp g rho1 v"
+    from xin[unfolded collect_combine_pp_def]
+    obtain c ex ret s t where
+      h: "(c, ex, ret) \<in> combines g" "ret = v"
+      and st: "s \<in> rho1 c" "t \<in> rho1 ex"
+      and x: "x = combine_states s t"
+      by blast
+    have "s \<in> rho2 c" "t \<in> rho2 ex" using st sub by auto
+    thus "x \<in> collect_combine_pp g rho2 v"
+      unfolding collect_combine_pp_def x using h by blast
+  qed
+qed
+
+lemma cfg_collect_ip_F_mono:
+  "mono (cfg_collect_ip_F g S)"
+proof (rule monoI)
+  fix rho1 rho2 :: cenv
+  assume le: "rho1 \<le> rho2"
+  show "cfg_collect_ip_F g S rho1 \<le> cfg_collect_ip_F g S rho2"
+  proof (rule le_funI)
+    fix v
+    show "cfg_collect_ip_F g S rho1 v \<subseteq> cfg_collect_ip_F g S rho2 v"
+      unfolding cfg_collect_ip_F_def
+      using monoD[OF collect_pp_mono[of g v] le]
+            monoD[OF collect_combine_pp_mono[of g v] le]
+      by (auto dest: subsetD)
+  qed
+qed
+
+lemma cfg_collect_ip_F_mono_S:
+  "S \<subseteq> S' \<Longrightarrow> cfg_collect_ip_F g S rho \<le> cfg_collect_ip_F g S' rho"
+  unfolding cfg_collect_ip_F_def le_fun_def by auto
+
+lemma cfg_collect_ip_mono_S:
+  "S \<subseteq> S' \<Longrightarrow> cfg_collect_ip g S \<le> cfg_collect_ip g S'"
+  unfolding cfg_collect_ip_def
+  by (rule lfp_mono) (rule cfg_collect_ip_F_mono_S)
+
+lemma cfg_collect_ip_lfp_unfold:
+  "cfg_collect_ip g S = cfg_collect_ip_F g S (cfg_collect_ip g S)"
+  unfolding cfg_collect_ip_def
+  by (simp add: cfg_collect_ip_F_mono def_lfp_unfold)
+
+(* -- Relation to intra-procedural cfg_collect ---------------------- *)
+
+lemma collect_combine_pp_empty[simp]:
+  "combines g = {} \<Longrightarrow> collect_combine_pp g rho v = {}"
+  unfolding collect_combine_pp_def by auto
+
+lemma cfg_collect_ip_F_eq_cfg_collect_F:
+  assumes "combines g = {}"
+  shows "cfg_collect_ip_F g S rho v = cfg_collect_F g S rho v"
+  unfolding cfg_collect_ip_F_def cfg_collect_F_def using assms by auto
+
+lemma cfg_collect_ip_eq_cfg_collect:
+  assumes "combines g = {}"
+  shows "cfg_collect_ip g S = cfg_collect g S"
+proof -
+  have eq: "cfg_collect_ip_F g S = cfg_collect_F g S"
+  proof
+    fix rho
+    show "cfg_collect_ip_F g S rho = cfg_collect_F g S rho"
+    proof (rule ext)
+      fix v
+      show "cfg_collect_ip_F g S rho v = cfg_collect_F g S rho v"
+        using cfg_collect_ip_F_eq_cfg_collect_F[OF assms] .
+    qed
+  qed
+  show ?thesis unfolding cfg_collect_ip_def cfg_collect_def eq by simp
+qed
+
+lemma cfg_collect_ip_F_ge_cfg_collect_F:
+  "cfg_collect_F g S rho v \<subseteq> cfg_collect_ip_F g S rho v"
+  unfolding cfg_collect_F_def cfg_collect_ip_F_def by auto
+
+lemma cfg_collect_le_cfg_collect_ip:
+  "cfg_collect g S \<le> cfg_collect_ip g S"
+  unfolding cfg_collect_def cfg_collect_ip_def
+  by (simp add: cfg_collect_ip_F_ge_cfg_collect_F le_funI lfp_mono)
+ 
+
+lemma cfg_collect_ip_entry:
+  "S \<subseteq> cfg_collect_ip g S (cfg_entry g)"
+  by (smt (verit, best) Un_upper1 cfg_collect_F_def cfg_collect_ip_F_ge_cfg_collect_F
+      cfg_collect_ip_lfp_unfold order_trans)
+
+lemma cfg_collect_ip_post:
+  "cfg_collect_ip_F g S (cfg_collect_ip g S) v \<subseteq> cfg_collect_ip g S v"
+proof -
+  have eq: "cfg_collect_ip_F g S (cfg_collect_ip g S) v = cfg_collect_ip g S v"
+    using cfg_collect_ip_lfp_unfold by (simp add: le_fun_def)
+  show ?thesis by (simp add: eq)
+qed
+
+lemma collect_combine_pp_member:
+  assumes "(c, ex, ret) \<in> combines g" "ret = v"
+      and "s \<in> rho c" "t \<in> rho ex"
+  shows "combine_states s t \<in> collect_combine_pp g rho v"
+  using assms unfolding collect_combine_pp_def by blast
+
+lemma collect_combine_pp_in_cfg_collect_ip:
+  assumes le: "rho \<le> cfg_collect_ip g S"
+  shows "collect_combine_pp g rho v \<subseteq> cfg_collect_ip g S v"
+proof
+  fix x
+  assume xin: "x \<in> collect_combine_pp g rho v"
+  from xin obtain c ex ret s t where
+        h: "(c, ex, ret) \<in> combines g" "ret = v"
+    and st: "s \<in> rho c" "t \<in> rho ex"
+    and x: "x = combine_states s t"
+    unfolding collect_combine_pp_def by blast
+  from le have sc: "s \<in> cfg_collect_ip g S c" and tc: "t \<in> cfg_collect_ip g S ex"
+    unfolding le_fun_def using st by auto
+  have mem: "combine_states s t \<in> collect_combine_pp g (cfg_collect_ip g S) v"
+  proof (rule collect_combine_pp_member)
+    show "(c, ex, ret) \<in> combines g" using h by simp
+    show "ret = v" using h by simp
+    show "s \<in> cfg_collect_ip g S c" using sc .
+    show "t \<in> cfg_collect_ip g S ex" using tc .
+  qed
+  have step: "combine_states s t \<in> cfg_collect_ip_F g S (cfg_collect_ip g S) v"
+    unfolding cfg_collect_ip_F_def using mem by auto
+  show "x \<in> cfg_collect_ip g S v"
+    using x step cfg_collect_ip_post by blast
+qed
+
+
+end
