src/Equations/Constraint_System_IP_Sound.thy
@@ -1,0 +1,208 @@
+theory Constraint_System_IP_Sound
+  imports Constraint_System_Sound CFG_Collect_IP
+begin
+
+(* Interprocedural soundness (M1 slice 3, L-sound'). *)
+
+lemma apply_tf_le_rhs_ip:
+  fixes g :: cfg and tf :: "'a::bounded_semilattice_sup_bot domain_transfer"
+    and env :: "pp \<Rightarrow> 'a abs_state" and s0 :: "'a abs_state"
+  assumes fin: "finite (edges g)"
+  assumes finC: "finite (combines g)"
+  assumes uav: "(u, a, v) \<in> edges g"
+  shows "apply_tf tf a (env u) \<le> rhs_ip g tf (\<squnion>) bot s0 env v"
+  using apply_tf_le_rhs[OF fin uav] rhs_le_rhs_ip[OF fin finC] by (rule order_trans)
+
+lemma combine_abs_le_rhs_ip:
+  fixes g :: cfg and tf :: "'a::bounded_semilattice_sup_bot domain_transfer"
+    and env :: "pp \<Rightarrow> 'a abs_state" and s0 :: "'a abs_state"
+  assumes finE: "finite (edges g)"
+  assumes finC: "finite (combines g)"
+  assumes uce: "(c, e, v) \<in> combines g"
+  shows "combine_abs (env c) (env e) \<le> rhs_ip g tf (\<squnion>) bot s0 env v"
+proof -
+  define C :: "(pp \<times> pp) set"
+    where "C = {(c', e'). (c', e', v) \<in> combines g}"
+  define f where "f \<equiv> \<lambda>(c', e'). combine_abs (env c') (env e')"
+  have finCset: "finite C"
+    unfolding C_def using finC finite_combine_predecessors
+    by (simp add: combine_predecessors_def)
+  define edge_vals where
+    "edge_vals = image (\<lambda>(u, a). apply_tf tf a (env u)) (predecessors g v)"
+  define comb_vals where
+    "comb_vals = image (\<lambda>(c', e'). combine_abs (env c') (env e')) (combine_predecessors g v)"
+  define base where
+    "base = (if v = cfg_entry g then insert s0 (edge_vals \<union> comb_vals)
+            else edge_vals \<union> comb_vals)"
+  have fin_edge: "finite edge_vals"
+    unfolding edge_vals_def using finE by (simp add: finite_predecessors)
+  have fin_comb: "finite comb_vals"
+    unfolding comb_vals_def using finC by (simp add: finite_combine_predecessors)
+  have fin_base: "finite base"
+    unfolding base_def using fin_edge fin_comb by simp
+  have mem_base: "combine_abs (env c) (env e) \<in> base"
+    using uce unfolding base_def comb_vals_def combine_predecessors_def by auto
+  show ?thesis
+  proof -
+    have "combine_abs (env c) (env e) \<le> abs_join_set (\<squnion>) bot base"
+      using sup_fold_ge_state[OF fin_base mem_base] unfolding abs_join_set_def by simp    also have "... = rhs_ip g tf (\<squnion>) bot s0 env v"
+      unfolding rhs_ip_def Let_def base_def edge_vals_def comb_vals_def
+        predecessors_def combine_predecessors_def
+      by simp
+    finally show ?thesis .
+  qed
+
+qed
+
+context sound_domain
+begin
+
+lemma combine_states_sound:
+  assumes sc: "s \<in> gamma_state \<sigma>c" and se: "t \<in> gamma_state \<sigma>e"
+  shows "combine_states s t \<in> gamma_state (combine_abs \<sigma>c \<sigma>e)"
+proof -
+  from sc have Vc: "\<forall>z. s z \<in> gamma (\<sigma>c z)"
+    unfolding gamma_state_def by auto
+  from se have Ve: "\<forall>z. t z \<in> gamma (\<sigma>e z)"
+    unfolding gamma_state_def by auto
+  show ?thesis unfolding gamma_state_def combine_abs_def combine_states_def
+    using Vc Ve by auto
+  
+qed
+
+lemma collect_pp_abstract_sound_ip:
+  assumes fin: "finite (edges g)"
+  assumes finC: "finite (combines g)"
+  assumes post_fp: "is_post_fixpoint_ip g tf (\<squnion>) bot s0 env"
+  assumes tf_sound_assign:
+    "\<forall>x a sigma. \<forall>s \<in> gamma_state sigma.
+       s(x := aval a s) \<in> gamma_state (tf_assign tf x a sigma)"
+  assumes tf_sound_assume:
+    "\<forall>b sigma. \<forall>s \<in> gamma_state sigma. bval b s
+       \<longrightarrow> s \<in> gamma_state (tf_assume tf b sigma)"
+  assumes tf_sound_assume_not:
+    "\<forall>b sigma. \<forall>s \<in> gamma_state sigma. \<not> bval b s
+       \<longrightarrow> s \<in> gamma_state (tf_assume_not tf b sigma)"
+  assumes tf_sound_enter:
+    "\<forall>sigma. \<forall>s \<in> gamma_state sigma.
+       enter_state s \<in> gamma_state (tf_enter tf sigma)"
+  shows "collect_pp g (\<lambda>v. gamma_state (env v)) v \<subseteq> gamma_state (env v)"
+proof
+  fix x
+  assume xin: "x \<in> collect_pp g (\<lambda>v. gamma_state (env v)) v"
+  then obtain u a where uav: "(u, a, v) \<in> edges g"
+    and xin': "x \<in> edge_collect a (gamma_state (env u))"
+    unfolding collect_pp_def by blast
+  have step1: "x \<in> gamma_state (apply_tf tf a (env u))"
+    using edge_collect_apply_tf_sound[OF tf_sound_assign tf_sound_assume
+            tf_sound_assume_not tf_sound_enter] xin' by blast
+  have le_rhs: "apply_tf tf a (env u) \<le> rhs_ip g tf (\<squnion>) bot s0 env v"
+    by (rule apply_tf_le_rhs_ip[OF fin finC uav])
+  have le_env: "rhs_ip g tf (\<squnion>) bot s0 env v \<le> env v"
+    using post_fp unfolding is_post_fixpoint_ip_def by simp
+  show "x \<in> gamma_state (env v)"
+    using gamma_state_mono[OF order_trans[OF le_rhs le_env]] step1 by blast
+qed
+
+lemma collect_combine_pp_abstract_sound:
+  assumes fin: "finite (edges g)"
+  assumes finC: "finite (combines g)"
+  assumes post_fp: "is_post_fixpoint_ip g tf (\<squnion>) bot s0 env"
+  assumes tf_sound_assign:
+    "\<forall>x a sigma. \<forall>s \<in> gamma_state sigma.
+       s(x := aval a s) \<in> gamma_state (tf_assign tf x a sigma)"
+  assumes tf_sound_assume:
+    "\<forall>b sigma. \<forall>s \<in> gamma_state sigma. bval b s
+       \<longrightarrow> s \<in> gamma_state (tf_assume tf b sigma)"
+  assumes tf_sound_assume_not:
+    "\<forall>b sigma. \<forall>s \<in> gamma_state sigma. \<not> bval b s
+       \<longrightarrow> s \<in> gamma_state (tf_assume_not tf b sigma)"
+  assumes tf_sound_enter:
+    "\<forall>sigma. \<forall>s \<in> gamma_state sigma.
+       enter_state s \<in> gamma_state (tf_enter tf sigma)"
+  shows "collect_combine_pp g (\<lambda>v. gamma_state (env v)) v
+         \<subseteq> gamma_state (env v)"
+proof
+  fix x
+  assume xin: "x \<in> collect_combine_pp g (\<lambda>v. gamma_state (env v)) v"
+  from xin obtain c ex ret s t where
+        h: "(c, ex, ret) \<in> combines g" "ret = v"
+    and st: "s \<in> gamma_state (env c)" "t \<in> gamma_state (env ex)"
+    and x: "x = combine_states s t"
+    unfolding collect_combine_pp_def by blast
+  have step: "x \<in> gamma_state (combine_abs (env c) (env ex))"
+    using combine_states_sound[OF st] x by simp
+  have uce: "(c, ex, v) \<in> combines g"
+    using h(1,2) by force
+  have le_rhs: "combine_abs (env c) (env ex) \<le> rhs_ip g tf (\<squnion>) bot s0 env v"
+    by (rule combine_abs_le_rhs_ip[OF fin finC uce])
+  have le_env: "rhs_ip g tf (\<squnion>) bot s0 env v \<le> env v"
+    using post_fp unfolding is_post_fixpoint_ip_def by simp
+  show "x \<in> gamma_state (env v)"
+    using gamma_state_mono[OF order_trans[OF le_rhs le_env]] step by blast
+qed
+
+lemma s0_le_rhs_ip_entry:
+  fixes g :: cfg and tf :: "'a::bounded_semilattice_sup_bot domain_transfer"
+    and env :: "pp \<Rightarrow> 'a abs_state" and s0 :: "'a abs_state"
+  assumes fin: "finite (edges g)"
+  assumes finC: "finite (combines g)"
+  shows "s0 \<le> rhs_ip g tf (\<squnion>) bot s0 env (cfg_entry g)"
+proof -
+  have "s0 \<le> rhs g tf (\<squnion>) bot s0 env (cfg_entry g)"
+    by (rule s0_le_rhs_entry[OF fin])
+  also have "rhs g tf (\<squnion>) bot s0 env (cfg_entry g)
+             \<le> rhs_ip g tf (\<squnion>) bot s0 env (cfg_entry g)"
+    by (rule rhs_le_rhs_ip[OF fin finC])
+  finally show ?thesis .
+qed
+
+theorem post_fixpoint_sound_ip:
+  assumes fin: "finite (edges g)"
+  assumes finC: "finite (combines g)"
+  assumes post_fp: "is_post_fixpoint_ip g tf (\<squnion>) bot s0 env"
+  assumes S_sound: "S \<le> gamma_state s0"
+  assumes tf_sound_assign:
+    "\<forall>x a sigma. \<forall>s \<in> gamma_state sigma.
+       s(x := aval a s) \<in> gamma_state (tf_assign tf x a sigma)"
+  assumes tf_sound_assume:
+    "\<forall>b sigma. \<forall>s \<in> gamma_state sigma. bval b s
+       \<longrightarrow> s \<in> gamma_state (tf_assume tf b sigma)"
+  assumes tf_sound_assume_not:
+    "\<forall>b sigma. \<forall>s \<in> gamma_state sigma. \<not> bval b s
+       \<longrightarrow> s \<in> gamma_state (tf_assume_not tf b sigma)"
+  assumes tf_sound_enter:
+    "\<forall>sigma. \<forall>s \<in> gamma_state sigma.
+       enter_state s \<in> gamma_state (tf_enter tf sigma)"
+  shows "\<forall>v. cfg_collect_ip g S v \<le> gamma_state (env v)"
+proof -
+  have coll_le: "\<And>v. collect_pp g (\<lambda>v. gamma_state (env v)) v \<le> gamma_state (env v)"
+    by (rule collect_pp_abstract_sound_ip[OF fin finC post_fp
+              tf_sound_assign tf_sound_assume tf_sound_assume_not tf_sound_enter])
+  have comb_le: "\<And>v. collect_combine_pp g (\<lambda>v. gamma_state (env v)) v
+                  \<le> gamma_state (env v)"
+    by (rule collect_combine_pp_abstract_sound[OF fin finC post_fp
+              tf_sound_assign tf_sound_assume tf_sound_assume_not tf_sound_enter])
+  have s0_le_env: "s0 \<le> env (cfg_entry g)"
+    using s0_le_rhs_ip_entry[OF fin finC]
+          post_fp[unfolded is_post_fixpoint_ip_def, rule_format, of "cfg_entry g"]
+    by (rule order_trans)
+  have S_le_env: "S \<le> gamma_state (env (cfg_entry g))"
+    using S_sound gamma_state_mono[OF s0_le_env] by blast
+  have key: "cfg_collect_ip_F g S (\<lambda>v. gamma_state (env v)) \<le> (\<lambda>v. gamma_state (env v))"
+  proof (rule le_funI)
+    fix v
+    show "cfg_collect_ip_F g S (\<lambda>v. gamma_state (env v)) v \<le> gamma_state (env v)"
+      unfolding cfg_collect_ip_F_def
+      using coll_le comb_le S_le_env by auto
+  qed
+  have "cfg_collect_ip g S \<le> (\<lambda>v. gamma_state (env v))"
+    unfolding cfg_collect_ip_def
+    by (simp add: key lfp_lowerbound)
+ 
+  then show ?thesis by (auto simp: le_fun_def)
+qed
+
+end
+
+end
